end of day 06/02/19

inference-tool/src/main/scala/inference/DataType.scala
@@ -1,4 +1,0 @@
-object DataType extends Enumeration {
-  type DataType = Value
-  val NUM, STR, UNBOUND = Value
-}
