formal/inference/General_Subsumption.thy
@@ -1,0 +1,111 @@
+theory General_Subsumption
+imports "../Contexts" Trace_Matches
+begin
+
+lemma ctx_simp: "(\<lambda>r. and (if r = V (I i) then snd (V (I i), cexp.Eq s) else cexp.Bc True) (\<lbrakk>\<rbrakk> r)) = \<lbrakk>V (I i) \<mapsto> Eq s\<rbrakk>"
+  apply (rule ext)
+  by simp
+
+lemma generalise_subsumption: "subsumes \<lbrakk>\<rbrakk> \<lparr>Label=l, Arity=a, Guard=[], Outputs=[], Updates=[(R r, (V (I i)))]\<rparr> 
+                  \<lparr>Label=l, Arity=a, Guard=[GExp.Eq (V (I i)) (L s)], Outputs=[], Updates=[]\<rparr>"
+  apply (simp add: subsumes_def)
+  apply standard
+   apply clarify
+   apply (case_tac "cval (\<lbrakk>\<rbrakk> r) ia")
+    apply simp
+   apply simp
+
+  apply standard
+   apply clarify
+   apply (simp add: posterior_def Let_def ctx_simp)
+   apply (case_tac "consistent \<lbrakk>V (I i) \<mapsto> cexp.Eq s\<rbrakk>")
+    apply (simp add: remove_input_constraints_def)
+    apply (case_tac "constrains_an_input ra")
+     apply simp
+    apply simp
+    apply (case_tac "ra = V (R r)")
+     apply simp
+    apply (case_tac "ra = V (I i)")
+     apply simp
+    apply simp
+   apply simp
+   apply (simp add: posterior_def Let_def ctx_simp)
+  apply standard
+   apply (simp add: consistent_def remove_input_constraints_def consistent_empty_4)
+  by (simp add: inconsistent_false)
+
+lemma incoming_transition_alt_def: "incoming_transition_to e n = (\<exists>t from. ((from, n), t) |\<in>| e)"
+  apply (simp add: incoming_transition_to_def)
+  apply (simp add: ffilter_def fset_both_sides Abs_fset_inverse)
+  apply (simp add: fmember_def)
+  apply (simp add: Set.filter_def)
+  by auto
+
+lemma no_step_to: "\<not> incoming_transition_to t m \<Longrightarrow>
+       step t n r aa b \<noteq> Some (uw, m, ux, r')"
+  apply (simp add: incoming_transition_alt_def step_def)
+  apply safe
+  apply (case_tac "fthe_elem (possible_steps t n r aa b)")
+  apply simp
+  using singleton_dest by blast
+
+lemma no_route_to_no_access: "\<not> incoming_transition_to t 0 \<Longrightarrow> \<forall>r s. s \<noteq> 0 \<longrightarrow> \<not>gets_us_to 0 t s r p"
+proof(induct p)
+  case Nil
+  then show ?case
+    by (simp add: no_further_steps)
+next
+  case (Cons a p)
+  then show ?case
+    apply clarify
+    apply (rule gets_us_to.cases)
+       apply simp
+      apply simp
+     apply clarify
+     apply simp
+     apply (metis no_step_to Cons.hyps)
+    by simp
+qed
+
+lemma no_return_to_initial: "\<not> incoming_transition_to t 0 \<Longrightarrow> accepts_trace t p \<and> gets_us_to 0 t 0 Map.empty p \<Longrightarrow> p = []"
+proof(induct p)
+  case Nil
+  then show ?case
+    by simp
+next
+  case (Cons a p)
+  then show ?case
+    apply (simp add: accepts_trace_def)
+    apply (rule gets_us_to.cases)
+       apply auto[1]
+      apply simp
+     apply clarify
+     apply simp
+     apply (case_tac "s' = 0")
+      apply (simp add: no_step_to)
+     apply (simp add: no_route_to_no_access)
+    apply clarify
+    by (simp add: no_step_none)
+qed
+
+lemma anterior_context_no_return_to_zero: "\<not> incoming_transition_to t 0 \<Longrightarrow> accepts_trace t p \<and> gets_us_to 0 t 0 Map.empty p \<longrightarrow> anterior_context t' p = \<lbrakk>\<rbrakk>"
+proof(induct p)
+  case Nil
+  then show ?case
+    by (simp add: anterior_context_def)
+next
+  case (Cons a p)
+  then show ?case
+    using no_return_to_initial
+    by auto
+qed
+
+
+lemma "\<not> incoming_transition_to t 0 \<Longrightarrow> directly_subsumes t t' 0 \<lparr>Label=l, Arity=a, Guard=[], Outputs=[], Updates=[(R r, (V (I i)))]\<rparr> 
+                  \<lparr>Label=l, Arity=a, Guard=[GExp.Eq (V (I i)) (L s)], Outputs=[], Updates=[]\<rparr>"
+  apply (simp add: directly_subsumes_def anterior_context_no_return_to_zero)
+  apply (simp add: generalise_subsumption)
+  using generalise_subsumption
+  by blast
+
+end
